\documentclass{article}
\usepackage{hyperref}
\usepackage[linguistics]{forest}
\usepackage{graphicx}
\usepackage[margin=1in]{geometry}
\usepackage{adjustbox}
\usepackage{bookmark}
\usepackage{rotating}
\usepackage{amsmath, bm, amssymb}
\usepackage{amsthm}

\begin{document}
\thispagestyle{empty}
\begin{center}
    {\large\bf STAT 672}    \\*[5pt] {\Large Statistical Learning II}
    \\*[12pt] {\large John Karasev}
    \\ {\large Homework 2}
    \\ {\large January 31, 2020}
\end{center}
\section{Kernel centering}

Let $\mathcal{X}$ be a non empty set, $K$ a kernel over $\mathcal{X}$ and $H$ the 
RKHS with kernel $K$. Let $x_1,\ldots,x_n$, be $n$ points in $\mathcal{X}$.
Let $K_c$ like ``K centered\rq\rq{} be another kernel over $\mathcal{X}$ defined by 

\begin{equation}
    K_c(x,y)=\langle K(.,x)- \bar{f}(.), K(.,y)-\bar{f}(.)\rangle_H 
    \mbox{, with } \bar{f}(.)=\frac{1}{n}\sum_{i=1}^n K(.,x_i)
\end{equation}

\begin{enumerate}
    


    \item Verify that $K_c$ is a positive definite kernel; \\ 
          Let $H_c$ be the RKHS with reproducing kernel $K_c$. 

        \begin{proof}
        \begin{equation}
            \begin{aligned} 
                \mbox{for any $n$ in $\mathbb{N}$, $(a_1, ..., a_n)$ in $\mathbb{R}^n$ ,} \notag \\
                (x_1, ..., x_n) \in \mathbb{X}^n \\
                &\sum_{i,j=1}^{n} a_i a_j K_c(x_i, x_j)  \\
                &= \sum_{i,j=1}^{n} a_i a_j \langle K(.,x_i) - \bar{f}(.), K(.,x_j) - \bar{f}(.)\rangle_{\mathcal{H}} \\
                &= \bigg \langle \sum_{i=1}^{n} a_i [K(.,x_i) - \bar{f}(.)], 
                    \sum_{j=1}^{n} a_j [K(.,x_j) - \bar{f}(.)] \bigg \rangle_{\mathcal{H}} \\
                & = \bigg \| \sum_{i=1}^{n} a_i [K(.,x_i) - \bar{f}(.)] \bigg \|_{\mathcal{H}} \ge 0
            \end{aligned}
        \end{equation} 
        \end{proof}
    


    \item (**) Verify that for any $f \in H_c$, 
        
        \begin{equation}
            \frac{1}{n} \sum_{l=1}^n f(x_l)=0
        \end{equation}
        \[f(x) = \sum_{m=1}^n \alpha_m K_c(x,y_m) \notag \]
        \begin{proof}
        \begin{equation} 
            \begin{aligned} 
                \frac{1}{n} \sum_{l=1}^n f(x_l) &=0 \notag \\
                \frac{1}{n} \sum_{l=1}^n \sum_{m=1}^n \alpha_m K_c(x_l,y_m) &=0 \\
                \frac{1}{n} \sum_{l=1}^n \sum_{m=1}^n \alpha_m \bigg \langle K(.,x_l)- \frac{1}{n}\sum_{i=1}^n K(.,x_i), 
                    K(.,y_m)-\frac{1}{n}\sum_{i=1}^n K(.,x_i) \bigg \rangle_{\mathcal{H}}  &=0 \\
                \frac{1}{n} \bigg \langle \sum_{l=1}^n K(.,x_l)- \sum_{l=1}^n \frac{1}{n}\sum_{i=1}^n K(.,x_i), 
                    \sum_{m=1}^n \alpha_m K(.,y_m)-\sum_{m=1}^n \alpha_m \frac{1}{n}\sum_{i=1}^n K(.,x_i) \bigg \rangle_{\mathcal{H}}  &=0 \\
                \bigg \langle \sum_{l=1}^n K(.,x_l)- n \frac{1}{n}\sum_{i=1}^n K(.,x_i), 
                    \sum_{m=1}^n \frac{\alpha_m K(.,y_m)}{n}-\sum_{m=1}^n \frac{\alpha_m}{n}\sum_{i=1}^n \frac{K(.,x_i)}{n}  \bigg \rangle_{\mathcal{H}}  &=0 \\
                \bigg \langle 0, 
                    \sum_{m=1}^n \frac{\alpha_m K(.,y_m)}{n}-\sum_{m=1}^n \frac{\alpha_m}{n}\sum_{i=1}^n \frac{K(.,x_i)}{n}  \bigg \rangle_{\mathcal{H}}  &=0 \\
                    0&=0 \\
            \end{aligned} 
        \end{equation}
        \end{proof} 
        
        In homework 1, you have learned to sample functions from a RKHS with kernel $K$ over the set $\mathcal{X}=\{-m,\ldots,m\}$ according to the probability 
        
        \begin{equation}
            p(f)=Ce^{-\frac{||f||^2}{2}}
        \end{equation} 

        Here, you are asked to do the same thing but over the RKHS of a centered kernel $K_c$. 
        Specifically, choose  $m=10$, $n=11$, $x_1=-10,x_2=-9,\ldots,x_{11}=0$.

        \begin{equation} 
            \begin{aligned} 
                K_c(x,y) &= \bigg \langle K(.,x)- \frac{1}{n}\sum_{i=1}^n K(.,x_i), K(.,y)-\frac{1}{n}\sum_{i=1}^n K(.,x_i) \bigg \rangle \notag \\
                &= \bigg \langle K(.,x), K(.,y) \bigg \rangle + \bigg \langle K(.,x), \frac{1}{n} \sum_{i=i}^n K(.,x_i) \bigg \rangle + \\ 
                &\ \ \ \ \bigg \langle K(.,y), \frac{1}{n}\sum_{i=1}^{n} K(.,x_i) \bigg \rangle + 
                \bigg \langle \frac{1}{n} \sum_{i=1}^{n} K(.,x_i), \frac{1}{n}\sum_{j=1}^{n} K(.,x_j) \bigg \rangle \\ 
                & = K(x,y) + \frac{1}{n}\sum_{i=1}^{n}K(x,x_i) + \frac{1}{n} \sum_{i=1}^{n} K(y,x_i) + 
                \frac{1}{n^2} \sum_{i=1}^{n} \sum_{j=1}^{n} K(x_i, x_j) 
            \end{aligned} 
        \end{equation}

        \begin{enumerate}
            \item[Ex. 1] 
                \[K_c(x,y) = e^{\frac{-(x-y)^2}{2\tau}} - \frac{1}{11}\sum_{i=-10}^{0} e^{\frac{-(x-i)^2}{2\tau}}
                - \frac{1}{11}\sum_{i=-10}^{0} e^{\frac{-(y-i)^2}{2\tau}} + \frac{1}{121}\sum_{i=-10}^0\sum_{j=-10}^0 e^{\frac{-(i-j)^2}{2\tau}}\]
            \item[Ex 2.] 
                \[K_c(x,y) = (x y + 600)^2 - \frac{1}{11}\sum_{i=-10}^{0} (x i + 600)^2
                - \frac{1}{11}\sum_{i=-10}^{0} (y i + 600)^2 + \frac{1}{121}\sum_{i=-10}^0\sum_{j=-10}^0 (i j + 600)^2\]
            \item[Ex. 3] 
                \[K_c(x,y) = tanh(xy+1) - \frac{1}{11}\sum_{i=-10}^{0} tanh(xi+1)
                - \frac{1}{11}\sum_{i=-10}^{0} tanh(yi+1) + \frac{1}{121}\sum_{i=-10}^0\sum_{j=-10}^0 tanh(ij+1)\]
            \item[Ex. 4] 
                \[K_c(x,y) = [xy+50] - \frac{1}{11}\sum_{i=-10}^{0} [xi+50]
                - \frac{1}{11}\sum_{i=-10}^{0} [yi+50] + \frac{1}{121}\sum_{i=-10}^0\sum_{j=-10}^0 [ij+50]\]
        \end{enumerate} 

    \item (**) Write $K_c$ in term of $K$ using matrix operations. 
    


    \item Choose the Gaussian kernel with $\tau=10$, and show 10 samples. 
        
        \begin{equation}
            \frac{1}{11}\sum_{i=-10}^0 f(i)=0
        \end{equation}
        
        up to numerical errors.  



\end{enumerate}

\end{document}
